interface/Json3.fsti
@@ -1,4 +1,4 @@
-module Json
+module Json3
 
 module M = Dependent_map
 open FStar.Seq
@@ -7,6 +7,7 @@ module S = Set_extended
 type kt : eqtype =
   |Alpha_t : string -> kt
   |Beta_t : string -> kt
+  |Gamma_t : string -> kt
 
 //concrete state of alpha type
 val concrete_st_a : Type0
@@ -14,10 +15,14 @@ val concrete_st_a : Type0
 //concrete state of beta type
 val concrete_st_b : Type0
 
+//concrete state of gamma type
+val concrete_st_c : Type0
+
 let vt (c:kt) : Type0 =
   match c with
   |Alpha_t _ -> concrete_st_a
   |Beta_t _ -> concrete_st_b
+  |Gamma_t _ -> concrete_st_c
 
 //concrete state
 type concrete_st = M.t kt vt
@@ -28,10 +33,14 @@ val init_st_a : concrete_st_a
 //init state of beta type
 val init_st_b : concrete_st_b
 
+//init state of gamma type
+val init_st_c : concrete_st_c
+
 let init_st_v (k:kt) : vt k =
   match k with
   |Alpha_t _ -> init_st_a
   |Beta_t _ -> init_st_b
+  |Gamma_t _ -> init_st_c
 
 let init_st (k:kt) : concrete_st = M.const_on S.empty (fun k -> init_st_v k)
 
@@ -40,17 +49,21 @@ let sel (s:concrete_st) (k:kt) =
   match k with
   |Alpha_t _ -> if M.contains s k then M.sel s k else init_st_a
   |Beta_t _ -> if M.contains s k then M.sel s k else init_st_b
+  |Gamma_t _ -> if M.contains s k then M.sel s k else init_st_c
 
 val eq_a (a b:concrete_st_a) : Type0
 val eq_b (a b:concrete_st_b) : Type0
+val eq_c (a b:concrete_st_c) : Type0
 
 let eq (a b:concrete_st) =
   //M.equal a b
   //(forall k. M.contains a k = M.contains b k /\ sel a k == sel b k)
   (forall k. M.contains a (Alpha_t k) = M.contains b (Alpha_t k) /\ 
         M.contains a (Beta_t k) = M.contains b (Beta_t k) /\
+        M.contains a (Gamma_t k) = M.contains b (Gamma_t k) /\
         eq_a (sel a (Alpha_t k)) (sel b (Alpha_t k)) /\
-        eq_b (sel a (Beta_t k)) (sel b (Beta_t k)))
+        eq_b (sel a (Beta_t k)) (sel b (Beta_t k)) /\
+        eq_c (sel a (Gamma_t k)) (sel b (Gamma_t k)))
 
 val lem_eq_a (a b:concrete_st_a) 
   : Lemma (ensures eq_a a b <==> a == b)
@@ -59,6 +72,10 @@ val lem_eq_a (a b:concrete_st_a)
 val lem_eq_b (a b:concrete_st_b) 
   : Lemma (ensures eq_b a b <==> a == b)
           [SMTPat (eq_b a b)]
+          
+val lem_eq_c (a b:concrete_st_c) 
+  : Lemma (ensures eq_c a b <==> a == b)
+          [SMTPat (eq_c a b)]
           
 let symmetric (a b:concrete_st) 
   : Lemma (requires eq a b)
@@ -78,9 +95,13 @@ val app_op_a : eqtype
 //beta MRDT operation type
 val app_op_b : eqtype
 
+//gamma MRDT operation type
+val app_op_c : eqtype
+
 type app_op_v : eqtype =
   |Alpha_op : app_op_a -> app_op_v
   |Beta_op : app_op_b -> app_op_v
+  |Gamma_op : app_op_c -> app_op_v
 
 type app_op_t:eqtype =
   |Set : string (* key *) -> app_op_v (* value op *) -> app_op_t
@@ -89,6 +110,7 @@ type op_t = pos (*timestamp*) & (nat (*replica ID*) & app_op_t)
 type op_v = pos (*timestamp*) & (nat (*replica ID*) & app_op_v)
 type op_a = pos (*timestamp*) & (nat (*replica ID*) & app_op_a)
 type op_b = pos (*timestamp*) & (nat (*replica ID*) & app_op_b)
+type op_c = pos (*timestamp*) & (nat (*replica ID*) & app_op_c)
 
 let get_rid (_,(rid,_)) = rid
 
@@ -104,6 +126,11 @@ let is_beta_op (o:op_t) =
   |Set _ (Beta_op _) -> true
   |_ -> false
 
+let is_gamma_op (o:op_t) = 
+  match snd (snd o) with
+  |Set _ (Gamma_op _) -> true
+  |_ -> false
+  
 let get_op_a (o:op_t{is_alpha_op o}) : op_a =
   match o with
   |ts, (rid, Set _ (Alpha_op op)) -> (ts,(rid,op))
@@ -111,6 +138,10 @@ let get_op_a (o:op_t{is_alpha_op o}) : op_a =
 let get_op_b (o:op_t{is_beta_op o}) : op_b =
   match o with
   |ts, (rid, Set _ (Beta_op op)) -> (ts,(rid,op))
+
+let get_op_c (o:op_t{is_gamma_op o}) : op_c =
+  match o with
+  |ts, (rid, Set _ (Gamma_op op)) -> (ts,(rid,op))
   
 //do function of alpha type
 val do_a (s:concrete_st_a) (o:op_a) : concrete_st_a
@@ -118,15 +149,17 @@ val do_a (s:concrete_st_a) (o:op_a) : concrete_st_a
 //do function of beta type
 val do_b (s:concrete_st_b) (o:op_b) : concrete_st_b
 
+//do function of gamma type
+val do_c (s:concrete_st_c) (o:op_c) : concrete_st_c
+
 let get_key (_,(_,Set k _)) = k
 
 //do function of map
-let do (s:concrete_st) (o:op_t) 
-  : (r:concrete_st{(is_alpha_op o ==> (forall k. M.contains r k <==> M.contains s k \/ k = Alpha_t (get_key o))) /\
-                   (is_beta_op o ==> (forall k. M.contains r k <==> M.contains s k \/ k = Beta_t (get_key o)))}) =
+let do (s:concrete_st) (o:op_t) : concrete_st =
   match snd (snd o) with
   |Set k (Alpha_op _) -> let v = sel s (Alpha_t k) in M.upd s (Alpha_t k) (do_a v (get_op_a o))
   |Set k (Beta_op _) -> let v = sel s (Beta_t k) in M.upd s (Beta_t k) (do_b v (get_op_b o))
+  |Set k (Gamma_op _) -> let v = sel s (Gamma_t k) in M.upd s (Gamma_t k) (do_c v (get_op_c o))
 
 type rc_res =
   |Fst_then_snd //o1 -> o2
@@ -137,21 +170,26 @@ val rc_a (o1 o2:op_a) : rc_res
 
 val rc_b (o1 o2:op_b) : rc_res
 
+val rc_c (o1 o2:op_c) : rc_res
+
 //conflict resolution
 let rc (o1 o2:op_t) : rc_res = 
   match snd (snd o1), snd (snd o2) with
   |Set k1 (Alpha_op _), Set k2 (Alpha_op _) -> if k1 = k2 then rc_a (get_op_a o1) (get_op_a o2) else Either
   |Set k1 (Beta_op _), Set k2 (Beta_op _) -> if k1 = k2 then rc_b (get_op_b o1) (get_op_b o2) else Either
+  |Set k1 (Gamma_op _), Set k2 (Gamma_op _) -> if k1 = k2 then rc_c (get_op_c o1) (get_op_c o2) else Either
   |_ -> Either
 
 val merge_a (l a b:concrete_st_a) : concrete_st_a 
 
 val merge_b (l a b:concrete_st_b) : concrete_st_b
 
+val merge_c (l a b:concrete_st_c) : concrete_st_c
+
 let compose_values (k:kt) (l a b:concrete_st) : vt k =
-  if Alpha_t? k then 
-    merge_a (sel l k) (sel a k) (sel b k)
-  else merge_b (sel l k) (sel a k) (sel b k)
+  if Alpha_t? k then merge_a (sel l k) (sel a k) (sel b k)
+  else if Beta_t? k then merge_b (sel l k) (sel a k) (sel b k)
+  else merge_c (sel l k) (sel a k) (sel b k)
 
 // concrete merge operation
 let merge (l a b:concrete_st) : concrete_st =
@@ -159,12 +197,6 @@ let merge (l a b:concrete_st) : concrete_st =
   let u = M.const_on keys (fun k -> init_st k) in
   M.map (fun k _ -> compose_values k l a b) u
 
-let commutes_with_a (o1 o2:op_a) =
-  forall s. eq_a (do_a (do_a s o1) o2) (do_a (do_a s o2) o1)
-
-let commutes_with_b (o1 o2:op_b) =
-  forall s. eq_b (do_b (do_b s o1) o2) (do_b (do_b s o2) o1)
-  
 let commutes_with (o1 o2:op_t) =
   forall s. eq (do (do s o1) o2) (do (do s o2) o1)
 
@@ -207,6 +239,10 @@ val merge_comm_a (l a b: concrete_st_a)
 val merge_comm_b (l a b: concrete_st_b) 
   : Lemma (ensures eq_b (merge_b l a b) (merge_b l b a))
           [SMTPat (merge_b l a b)]
+
+val merge_comm_c (l a b: concrete_st_c) 
+  : Lemma (ensures eq_c (merge_c l a b) (merge_c l b a))
+          [SMTPat (merge_c l a b)]
           
 let merge_comm (l a b:concrete_st)
   : Lemma (ensures (eq (merge l a b) (merge l b a))) = ()
@@ -220,6 +256,10 @@ val merge_idem_b (s: concrete_st_b)
   : Lemma (ensures eq_b (merge_b s s s) s)
           [SMTPat (merge_b s s s)]
 
+val merge_idem_c (s: concrete_st_c) 
+  : Lemma (ensures eq_c (merge_c s s s) s)
+          [SMTPat (merge_c s s s)]
+          
 let merge_idem (s:concrete_st)
   : Lemma (ensures eq (merge s s s) s) = ()
 
@@ -240,11 +280,18 @@ val base_2op_b (o1 o2:op_b)
           (ensures eq_b (merge_b init_st_b (do_b init_st_b o1) (do_b init_st_b o2)) 
                         (do_b (merge_b init_st_b init_st_b (do_b init_st_b o2)) o1))
 
+val base_2op_c (o1 o2:op_c) 
+  : Lemma (requires (Fst_then_snd? (rc_c o2 o1) \/ Either? (rc_c o2 o1)) /\ get_rid o1 <> get_rid o2 /\
+                    distinct_ops o1 o2)
+          (ensures eq_c (merge_c init_st_c (do_c init_st_c o1) (do_c init_st_c o2)) 
+                        (do_c (merge_c init_st_c init_st_c (do_c init_st_c o2)) o1))
+                        
 val base_2op' (o1 o2:op_t) (t:kt)
   : Lemma (requires Either? (rc o2 o1) /\ get_rid o1 <> get_rid o2 /\ distinct_ops o1 o2 /\
                     ~ (get_key o1 = get_key o2 /\ 
                        is_alpha_op o1 /\ is_alpha_op o2 /\ (Fst_then_snd? (rc_a (get_op_a o2) (get_op_a o1)) || Either? (rc_a (get_op_a o2) (get_op_a o1))) /\
-                       is_beta_op o1 /\ is_beta_op o2 /\ (Fst_then_snd? (rc_b (get_op_b o2) (get_op_b o1)) || Either? (rc_b (get_op_b o2) (get_op_b o1)))))                
+                       is_beta_op o1 /\ is_beta_op o2 /\ (Fst_then_snd? (rc_b (get_op_b o2) (get_op_b o1)) || Either? (rc_b (get_op_b o2) (get_op_b o1))) /\
+                       is_gamma_op o1 /\ is_gamma_op o2 /\ (Fst_then_snd? (rc_c (get_op_c o2) (get_op_c o1)) || Either? (rc_c (get_op_c o2) (get_op_c o1)))))
           (ensures eq (merge (init_st t) (do (init_st t) o1) (do (init_st t) o2)) 
                       (do (merge (init_st t) (init_st t) (do (init_st t) o2)) o1))
 
@@ -257,6 +304,8 @@ let base_2op (o1 o2:op_t) (t:kt)
     base_2op_a (get_op_a o1) (get_op_a o2) 
   else if get_key o1 = get_key o2 && is_beta_op o1 && is_beta_op o2 then
     base_2op_b (get_op_b o1) (get_op_b o2) 
+  else if get_key o1 = get_key o2 && is_gamma_op o1 && is_gamma_op o2 then
+    base_2op_c (get_op_c o1) (get_op_c o2) 
   else if Either? (rc o2 o1) then base_2op' o1 o2 t
   else ()
 
@@ -272,26 +321,36 @@ val ind_lca_2op_b (l:concrete_st_b) (o1 o2 ol:op_b)
                     eq_b (merge_b l (do_b l o1) (do_b l o2)) (do_b (merge_b l l (do_b l o2)) o1))
           (ensures eq_b (merge_b (do_b l ol) (do_b (do_b l ol) o1) (do_b (do_b l ol) o2)) (do_b (merge_b (do_b l ol) (do_b l ol) (do_b (do_b l ol) o2)) o1))
 
+val ind_lca_2op_c (l:concrete_st_c) (o1 o2 ol:op_c)
+  : Lemma (requires (Fst_then_snd? (rc_c o2 o1) \/ Either? (rc_c o2 o1)) /\ get_rid o1 <> get_rid o2 /\
+                    distinct_ops o1 o2 /\ distinct_ops o1 ol /\ distinct_ops o2 ol /\
+                    eq_c (merge_c l (do_c l o1) (do_c l o2)) (do_c (merge_c l l (do_c l o2)) o1))
+          (ensures eq_c (merge_c (do_c l ol) (do_c (do_c l ol) o1) (do_c (do_c l ol) o2)) (do_c (merge_c (do_c l ol) (do_c l ol) (do_c (do_c l ol) o2)) o1))
+          
 val ind_lca_2op' (l:concrete_st) (o1 o2 ol:op_t)
   : Lemma (requires Either? (rc o2 o1) /\ get_rid o1 <> get_rid o2 /\
                     distinct_ops o1 o2 /\ distinct_ops o1 ol /\ distinct_ops o2 ol /\
                     ~ (get_key o1 = get_key ol && get_key o2 = get_key ol /\
                        is_alpha_op o1 /\ is_alpha_op o2 /\ is_alpha_op ol /\ (Fst_then_snd? (rc_a (get_op_a o2) (get_op_a o1)) || Either? (rc_a (get_op_a o2) (get_op_a o1))) /\
-                       is_beta_op o1 /\ is_beta_op o2 /\ is_beta_op ol /\ (Fst_then_snd? (rc_b (get_op_b o2) (get_op_b o1)) || Either? (rc_b (get_op_b o2) (get_op_b o1)))) /\
+                       is_beta_op o1 /\ is_beta_op o2 /\ is_beta_op ol /\ (Fst_then_snd? (rc_b (get_op_b o2) (get_op_b o1)) || Either? (rc_b (get_op_b o2) (get_op_b o1))) /\
+                       is_gamma_op o1 /\ is_gamma_op o2 /\ is_gamma_op ol /\ (Fst_then_snd? (rc_c (get_op_c o2) (get_op_c o1)) || Either? (rc_c (get_op_c o2) (get_op_c o1)))) /\
                     eq (merge l (do l o1) (do l o2)) (do (merge l l (do l o2)) o1))
           (ensures eq (merge (do l ol) (do (do l ol) o1) (do (do l ol) o2)) (do (merge (do l ol) (do l ol) (do (do l ol) o2)) o1))
 
+#set-options "--z3rlimit 100 --ifuel 3"
 let ind_lca_2op (l:concrete_st) (o1 o2 ol:op_t)
   : Lemma (requires (Fst_then_snd? (rc o2 o1) \/ Either? (rc o2 o1)) /\ get_rid o1 <> get_rid o2 /\
                     distinct_ops o1 o2 /\ distinct_ops o1 ol /\ distinct_ops o2 ol /\
                     eq (merge l (do l o1) (do l o2)) (do (merge l l (do l o2)) o1))
           (ensures eq (merge (do l ol) (do (do l ol) o1) (do (do l ol) o2)) (do (merge (do l ol) (do l ol) (do (do l ol) o2)) o1)) =
   let k = get_key ol in
-  let ka = Alpha_t k in let kb = Beta_t k in
+  let ka = Alpha_t k in let kb = Beta_t k in let kc = Gamma_t k in 
   if get_key o1 = k && get_key o2 = k && is_alpha_op o1 && is_alpha_op o2 && is_alpha_op ol && (Fst_then_snd? (rc_a (get_op_a o2) (get_op_a o1)) || Either? (rc_a (get_op_a o2) (get_op_a o1))) then
       ind_lca_2op_a (sel l ka) (get_op_a o1) (get_op_a o2) (get_op_a ol)
   else if get_key o1 = k && get_key o2 = k && is_beta_op o1 && is_beta_op o2 && is_beta_op ol && (Fst_then_snd? (rc_b (get_op_b o2) (get_op_b o1)) || Either? (rc_b (get_op_b o2) (get_op_b o1))) then
       ind_lca_2op_b (sel l kb) (get_op_b o1) (get_op_b o2) (get_op_b ol)
+  else if get_key o1 = k && get_key o2 = k && is_gamma_op o1 && is_gamma_op o2 && is_gamma_op ol && (Fst_then_snd? (rc_c (get_op_c o2) (get_op_c o1)) || Either? (rc_c (get_op_c o2) (get_op_c o1))) then
+      ind_lca_2op_c (sel l kc) (get_op_c o1) (get_op_c o2) (get_op_c ol)
   else if Either? (rc o2 o1) then ind_lca_2op' l o1 o2 ol
   else ()
 
@@ -310,19 +369,28 @@ val inter_right_base_2op_b (l a b :concrete_st_b) (o1 o2 ob ol:op_b)
                     eq_b (merge_b l (do_b a o1) (do_b (do_b b ob) o2)) (do_b (merge_b l a (do_b (do_b b ob) o2)) o1) /\ //from ind_right_2op
                     eq_b (merge_b (do_b l ol) (do_b (do_b a ol) o1) (do_b (do_b b ol) o2)) (do_b (merge_b (do_b l ol) (do_b a ol) (do_b (do_b b ol) o2)) o1))
           (ensures eq_b (merge_b (do_b l ol) (do_b (do_b a ol) o1) (do_b (do_b (do_b b ob) ol) o2)) (do_b (merge_b (do_b l ol) (do_b a ol) (do_b (do_b (do_b b ob) ol) o2)) o1))
+
+val inter_right_base_2op_c (l a b :concrete_st_c) (o1 o2 ob ol:op_c)
+  : Lemma (requires (Fst_then_snd? (rc_c o2 o1) \/ Either? (rc_c o2 o1)) /\ get_rid o1 <> get_rid o2 /\ Fst_then_snd? (rc_c ob ol) /\ get_rid ob <> get_rid ol /\
+                    distinct_ops o1 o2 /\ distinct_ops o1 ob /\ distinct_ops o1 ol /\ distinct_ops o2 ob /\ distinct_ops o2 ol /\ distinct_ops ob ol /\
+                    eq_c (merge_c l (do_c a o1) (do_c b o2)) (do_c (merge_c l a (do_c b o2)) o1) /\ //from pre-cond of ind_right_2op
+                    eq_c (merge_c l (do_c a o1) (do_c (do_c b ob) o2)) (do_c (merge_c l a (do_c (do_c b ob) o2)) o1) /\ //from ind_right_2op
+                    eq_c (merge_c (do_c l ol) (do_c (do_c a ol) o1) (do_c (do_c b ol) o2)) (do_c (merge_c (do_c l ol) (do_c a ol) (do_c (do_c b ol) o2)) o1))
+          (ensures eq_c (merge_c (do_c l ol) (do_c (do_c a ol) o1) (do_c (do_c (do_c b ob) ol) o2)) (do_c (merge_c (do_c l ol) (do_c a ol) (do_c (do_c (do_c b ob) ol) o2)) o1))
           
 val inter_right_base_2op' (l a b :concrete_st) (o1 o2 ob ol:op_t)
   : Lemma (requires Either? (rc o2 o1) /\ get_rid o1 <> get_rid o2 /\ Fst_then_snd? (rc ob ol) /\ get_rid ob <> get_rid ol /\
                     distinct_ops o1 o2 /\ distinct_ops o1 ob /\ distinct_ops o1 ol /\ distinct_ops o2 ob /\ distinct_ops o2 ol /\ distinct_ops ob ol /\
                     ~ (get_key o1 = get_key ol && get_key o2 = get_key ol /\ get_key ob = get_key ol /\
                        is_alpha_op o1 /\ is_alpha_op o2 /\ is_alpha_op ob /\ is_alpha_op ol /\ (Fst_then_snd? (rc_a (get_op_a o2) (get_op_a o1)) || Either? (rc_a (get_op_a o2) (get_op_a o1))) /\ Fst_then_snd? (rc_a (get_op_a ob) (get_op_a ol)) /\
-                       is_beta_op o1 /\ is_beta_op o2 /\ is_beta_op ob /\ is_beta_op ol /\ (Fst_then_snd? (rc_b (get_op_b o2) (get_op_b o1)) || Either? (rc_b (get_op_b o2) (get_op_b o1))) /\ Fst_then_snd? (rc_b (get_op_b ob) (get_op_b ol))) /\
+                       is_beta_op o1 /\ is_beta_op o2 /\ is_beta_op ob /\ is_beta_op ol /\ (Fst_then_snd? (rc_b (get_op_b o2) (get_op_b o1)) || Either? (rc_b (get_op_b o2) (get_op_b o1))) /\ Fst_then_snd? (rc_b (get_op_b ob) (get_op_b ol)) /\
+                       is_gamma_op o1 /\ is_gamma_op o2 /\ is_gamma_op ob /\ is_gamma_op ol /\ (Fst_then_snd? (rc_c (get_op_c o2) (get_op_c o1)) || Either? (rc_c (get_op_c o2) (get_op_c o1))) /\ Fst_then_snd? (rc_c (get_op_c ob) (get_op_c ol))) /\
                     eq (merge l (do a o1) (do b o2)) (do (merge l a (do b o2)) o1) /\ //from pre-cond of ind_right_2op
                     eq (merge l (do a o1) (do (do b ob) o2)) (do (merge l a (do (do b ob) o2)) o1) /\ //from ind_right_2op
                     eq (merge (do l ol) (do (do a ol) o1) (do (do b ol) o2)) (do (merge (do l ol) (do a ol) (do (do b ol) o2)) o1))
           (ensures eq (merge (do l ol) (do (do a ol) o1) (do (do (do b ob) ol) o2)) (do (merge (do l ol) (do a ol) (do (do (do b ob) ol) o2)) o1))
 
-#set-options "--z3rlimit 100 --ifuel 3"
+#set-options "--z3rlimit 300 --ifuel 3"
 let inter_right_base_2op (l a b :concrete_st) (o1 o2 ob ol:op_t)
   : Lemma (requires (Fst_then_snd? (rc o2 o1) \/ Either? (rc o2 o1)) /\ get_rid o1 <> get_rid o2 /\ Fst_then_snd? (rc ob ol) /\ get_rid ob <> get_rid ol /\
                     distinct_ops o1 o2 /\ distinct_ops o1 ob /\ distinct_ops o1 ol /\ distinct_ops o2 ob /\ distinct_ops o2 ol /\ distinct_ops ob ol /\
@@ -331,11 +399,13 @@ let inter_right_base_2op (l a b :concrete_st) (o1 o2 ob ol:op_t)
                     eq (merge (do l ol) (do (do a ol) o1) (do (do b ol) o2)) (do (merge (do l ol) (do a ol) (do (do b ol) o2)) o1))
           (ensures eq (merge (do l ol) (do (do a ol) o1) (do (do (do b ob) ol) o2)) (do (merge (do l ol) (do a ol) (do (do (do b ob) ol) o2)) o1)) =
   let k = get_key ol in
-  let ka = Alpha_t k in let kb = Beta_t k in
+  let ka = Alpha_t k in let kb = Beta_t k in let kc = Gamma_t k in
   if get_key o1 = k && get_key o2 = k && get_key ob = k && is_alpha_op o1 && is_alpha_op o2 && is_alpha_op ob && is_alpha_op ol && (Fst_then_snd? (rc_a (get_op_a o2) (get_op_a o1)) || Either? (rc_a (get_op_a o2) (get_op_a o1))) && Fst_then_snd? (rc_a (get_op_a ob) (get_op_a ol)) then
       inter_right_base_2op_a (sel l ka) (sel a ka) (sel b ka) (get_op_a o1) (get_op_a o2) (get_op_a ob) (get_op_a ol)
   else if get_key o1 = k && get_key o2 = k && get_key ob = k && is_beta_op o1 && is_beta_op o2 && is_beta_op ob && is_beta_op ol && (Fst_then_snd? (rc_b (get_op_b o2) (get_op_b o1)) || Either? (rc_b (get_op_b o2) (get_op_b o1))) && Fst_then_snd? (rc_b (get_op_b ob) (get_op_b ol)) then
       inter_right_base_2op_b (sel l kb) (sel a kb) (sel b kb) (get_op_b o1) (get_op_b o2) (get_op_b ob) (get_op_b ol)
+  else if get_key o1 = k && get_key o2 = k && get_key ob = k && is_gamma_op o1 && is_gamma_op o2 && is_gamma_op ob && is_gamma_op ol && (Fst_then_snd? (rc_c (get_op_c o2) (get_op_c o1)) || Either? (rc_c (get_op_c o2) (get_op_c o1))) && Fst_then_snd? (rc_c (get_op_c ob) (get_op_c ol)) then
+      inter_right_base_2op_c (sel l kc) (sel a kc) (sel b kc) (get_op_c o1) (get_op_c o2) (get_op_c ob) (get_op_c ol)
   else if Either? (rc o2 o1) then inter_right_base_2op' l a b o1 o2 ob ol
   else ()
 
@@ -350,13 +420,20 @@ val inter_left_base_2op_b (l a b :concrete_st_b) (o1 o2 ob ol:op_b)
                     distinct_ops o1 o2 /\ distinct_ops o1 ob /\ distinct_ops o1 ol /\ distinct_ops o2 ob /\ distinct_ops o2 ol /\ distinct_ops ob ol /\
                     eq_b (merge_b (do_b l ol) (do_b (do_b a ol) o1) (do_b (do_b b ol) o2)) (do_b (merge_b (do_b l ol) (do_b a ol) (do_b (do_b b ol) o2)) o1))
           (ensures eq_b (merge_b (do_b l ol) (do_b (do_b (do_b a ob) ol) o1) (do_b (do_b b ol) o2)) (do_b (merge_b (do_b l ol) (do_b (do_b a ob) ol) (do_b (do_b b ol) o2)) o1))
-          
+
+val inter_left_base_2op_c (l a b :concrete_st_c) (o1 o2 ob ol:op_c)
+  : Lemma (requires (Fst_then_snd? (rc_c o2 o1) \/ Either? (rc_c o2 o1)) /\ get_rid o1 <> get_rid o2 /\ Fst_then_snd? (rc_c ob ol) /\ get_rid ob <> get_rid ol /\
+                    distinct_ops o1 o2 /\ distinct_ops o1 ob /\ distinct_ops o1 ol /\ distinct_ops o2 ob /\ distinct_ops o2 ol /\ distinct_ops ob ol /\
+                    eq_c (merge_c (do_c l ol) (do_c (do_c a ol) o1) (do_c (do_c b ol) o2)) (do_c (merge_c (do_c l ol) (do_c a ol) (do_c (do_c b ol) o2)) o1))
+          (ensures eq_c (merge_c (do_c l ol) (do_c (do_c (do_c a ob) ol) o1) (do_c (do_c b ol) o2)) (do_c (merge_c (do_c l ol) (do_c (do_c a ob) ol) (do_c (do_c b ol) o2)) o1))
+
 val inter_left_base_2op' (l a b :concrete_st) (o1 o2 ob ol:op_t)
   : Lemma (requires Either? (rc o2 o1) /\ get_rid o1 <> get_rid o2 /\ Fst_then_snd? (rc ob ol) /\ get_rid ob <> get_rid ol /\
                     distinct_ops o1 o2 /\ distinct_ops o1 ob /\ distinct_ops o1 ol /\ distinct_ops o2 ob /\ distinct_ops o2 ol /\ distinct_ops ob ol /\
                     ~ (get_key o1 = get_key ol && get_key o2 = get_key ol /\ get_key ob = get_key ol /\
                        is_alpha_op o1 /\ is_alpha_op o2 /\ is_alpha_op ob /\ is_alpha_op ol /\ (Fst_then_snd? (rc_a (get_op_a o2) (get_op_a o1)) || Either? (rc_a (get_op_a o2) (get_op_a o1))) /\ Fst_then_snd? (rc_a (get_op_a ob) (get_op_a ol)) /\
-                       is_beta_op o1 /\ is_beta_op o2 /\ is_beta_op ob /\ is_beta_op ol /\ (Fst_then_snd? (rc_b (get_op_b o2) (get_op_b o1)) || Either? (rc_b (get_op_b o2) (get_op_b o1))) /\ Fst_then_snd? (rc_b (get_op_b ob) (get_op_b ol))) /\
+                       is_beta_op o1 /\ is_beta_op o2 /\ is_beta_op ob /\ is_beta_op ol /\ (Fst_then_snd? (rc_b (get_op_b o2) (get_op_b o1)) || Either? (rc_b (get_op_b o2) (get_op_b o1))) /\ Fst_then_snd? (rc_b (get_op_b ob) (get_op_b ol)) /\
+                       is_gamma_op o1 /\ is_gamma_op o2 /\ is_gamma_op ob /\ is_gamma_op ol /\ (Fst_then_snd? (rc_c (get_op_c o2) (get_op_c o1)) || Either? (rc_c (get_op_c o2) (get_op_c o1))) /\ Fst_then_snd? (rc_c (get_op_c ob) (get_op_c ol))) /\
                     eq (merge (do l ol) (do (do a ol) o1) (do (do b ol) o2)) (do (merge (do l ol) (do a ol) (do (do b ol) o2)) o1))
           (ensures eq (merge (do l ol) (do (do (do a ob) ol) o1) (do (do b ol) o2)) (do (merge (do l ol) (do (do a ob) ol) (do (do b ol) o2)) o1))
 
@@ -366,11 +443,13 @@ let inter_left_base_2op (l a b :concrete_st) (o1 o2 ob ol:op_t)
                     eq (merge (do l ol) (do (do a ol) o1) (do (do b ol) o2)) (do (merge (do l ol) (do a ol) (do (do b ol) o2)) o1))
           (ensures eq (merge (do l ol) (do (do (do a ob) ol) o1) (do (do b ol) o2)) (do (merge (do l ol) (do (do a ob) ol) (do (do b ol) o2)) o1)) =
   let k = get_key ol in
-  let ka = Alpha_t k in let kb = Beta_t k in
+  let ka = Alpha_t k in let kb = Beta_t k in let kc = Gamma_t k in
   if get_key o1 = k && get_key o2 = k && get_key ob = k && is_alpha_op o1 && is_alpha_op o2 && is_alpha_op ob && is_alpha_op ol && (Fst_then_snd? (rc_a (get_op_a o2) (get_op_a o1)) || Either? (rc_a (get_op_a o2) (get_op_a o1))) && Fst_then_snd? (rc_a (get_op_a ob) (get_op_a ol)) then
       inter_left_base_2op_a (sel l ka) (sel a ka) (sel b ka) (get_op_a o1) (get_op_a o2) (get_op_a ob) (get_op_a ol)
   else if get_key o1 = k && get_key o2 = k && get_key ob = k && is_beta_op o1 && is_beta_op o2 && is_beta_op ob && is_beta_op ol && (Fst_then_snd? (rc_b (get_op_b o2) (get_op_b o1)) || Either? (rc_b (get_op_b o2) (get_op_b o1))) && Fst_then_snd? (rc_b (get_op_b ob) (get_op_b ol)) then
       inter_left_base_2op_b (sel l kb) (sel a kb) (sel b kb) (get_op_b o1) (get_op_b o2) (get_op_b ob) (get_op_b ol)
+  else if get_key o1 = k && get_key o2 = k && get_key ob = k && is_gamma_op o1 && is_gamma_op o2 && is_gamma_op ob && is_gamma_op ol && (Fst_then_snd? (rc_c (get_op_c o2) (get_op_c o1)) || Either? (rc_c (get_op_c o2) (get_op_c o1))) && Fst_then_snd? (rc_c (get_op_c ob) (get_op_c ol)) then
+      inter_left_base_2op_c (sel l kc) (sel a kc) (sel b kc) (get_op_c o1) (get_op_c o2) (get_op_c ob) (get_op_c ol)
   else if Either? (rc o2 o1) then inter_left_base_2op' l a b o1 o2 ob ol
   else ()
 
@@ -389,6 +468,14 @@ val inter_right_2op_b (l a b :concrete_st_b) (o1 o2 ob ol o:op_b)
                     get_rid o <> get_rid ol /\
                     eq_b (merge_b (do_b l ol) (do_b (do_b a ol) o1) (do_b (do_b (do_b b ob) ol) o2)) (do_b (merge_b (do_b l ol) (do_b a ol) (do_b (do_b (do_b b ob) ol) o2)) o1))
           (ensures eq_b (merge_b (do_b l ol) (do_b (do_b a ol) o1) (do_b (do_b (do_b (do_b b o) ob) ol) o2)) (do_b (merge_b (do_b l ol) (do_b a ol) (do_b (do_b (do_b (do_b b o) ob) ol) o2)) o1))
+
+val inter_right_2op_c (l a b :concrete_st_c) (o1 o2 ob ol o:op_c)
+  : Lemma (requires (Fst_then_snd? (rc_c o2 o1) \/ Either? (rc_c o2 o1)) /\ get_rid o1 <> get_rid o2 /\ Fst_then_snd? (rc_c ob ol) /\ get_rid ob <> get_rid ol /\
+                    (~ (Either? (rc_c o ob)) \/ Fst_then_snd? (rc_c o ol)) /\
+                    distinct_ops o1 o2 /\ distinct_ops o1 ob /\ distinct_ops o1 ol /\ distinct_ops o1 o /\ distinct_ops o2 ob /\ distinct_ops o2 ol /\ distinct_ops o2 o /\ distinct_ops ob ol /\ distinct_ops ob o /\ distinct_ops ol o /\
+                    get_rid o <> get_rid ol /\
+                    eq_c (merge_c (do_c l ol) (do_c (do_c a ol) o1) (do_c (do_c (do_c b ob) ol) o2)) (do_c (merge_c (do_c l ol) (do_c a ol) (do_c (do_c (do_c b ob) ol) o2)) o1))
+          (ensures eq_c (merge_c (do_c l ol) (do_c (do_c a ol) o1) (do_c (do_c (do_c (do_c b o) ob) ol) o2)) (do_c (merge_c (do_c l ol) (do_c a ol) (do_c (do_c (do_c (do_c b o) ob) ol) o2)) o1))
           
 val inter_right_2op' (l a b :concrete_st) (o1 o2 ob ol o:op_t)
   : Lemma (requires Either? (rc o2 o1) /\ get_rid o1 <> get_rid o2 /\ Fst_then_snd? (rc ob ol) /\ get_rid ob <> get_rid ol /\
@@ -397,7 +484,8 @@ val inter_right_2op' (l a b :concrete_st) (o1 o2 ob ol o:op_t)
                     get_rid o <> get_rid ol /\
                     ~ (get_key o1 = get_key o && get_key o2 = get_key o /\ get_key ob = get_key o /\ get_key ol = get_key o /\
                        is_alpha_op o1 /\ is_alpha_op o2 /\ is_alpha_op ob /\ is_alpha_op ol /\ is_alpha_op o /\ (Fst_then_snd? (rc_a (get_op_a o2) (get_op_a o1)) \/ Either? (rc_a (get_op_a o2) (get_op_a o1))) /\ Fst_then_snd? (rc_a (get_op_a ob) (get_op_a ol)) /\ (Fst_then_snd? (rc_a (get_op_a o) (get_op_a ob)) \/ Snd_then_fst? (rc_a (get_op_a o) (get_op_a ob)) \/ Fst_then_snd? (rc_a (get_op_a o) (get_op_a ol))) /\
-                       is_beta_op o1 /\ is_beta_op o2 /\ is_beta_op ob /\ is_beta_op ol /\ is_beta_op o /\ (Fst_then_snd? (rc_b (get_op_b o2) (get_op_b o1)) \/ Either? (rc_b (get_op_b o2) (get_op_b o1))) /\ Fst_then_snd? (rc_b (get_op_b ob) (get_op_b ol)) /\ (Fst_then_snd? (rc_b (get_op_b o) (get_op_b ob)) \/ Snd_then_fst? (rc_b (get_op_b o) (get_op_b ob)) \/ Fst_then_snd? (rc_b (get_op_b o) (get_op_b ol)))) /\
+                       is_beta_op o1 /\ is_beta_op o2 /\ is_beta_op ob /\ is_beta_op ol /\ is_beta_op o /\ (Fst_then_snd? (rc_b (get_op_b o2) (get_op_b o1)) \/ Either? (rc_b (get_op_b o2) (get_op_b o1))) /\ Fst_then_snd? (rc_b (get_op_b ob) (get_op_b ol)) /\ (Fst_then_snd? (rc_b (get_op_b o) (get_op_b ob)) \/ Snd_then_fst? (rc_b (get_op_b o) (get_op_b ob)) \/ Fst_then_snd? (rc_b (get_op_b o) (get_op_b ol))) /\
+                       is_gamma_op o1 /\ is_gamma_op o2 /\ is_gamma_op ob /\ is_gamma_op ol /\ is_gamma_op o /\ (Fst_then_snd? (rc_c (get_op_c o2) (get_op_c o1)) \/ Either? (rc_c (get_op_c o2) (get_op_c o1))) /\ Fst_then_snd? (rc_c (get_op_c ob) (get_op_c ol)) /\ (Fst_then_snd? (rc_c (get_op_c o) (get_op_c ob)) \/ Snd_then_fst? (rc_c (get_op_c o) (get_op_c ob)) \/ Fst_then_snd? (rc_c (get_op_c o) (get_op_c ol)))) /\
                     eq (merge (do l ol) (do (do a ol) o1) (do (do (do b ob) ol) o2)) (do (merge (do l ol) (do a ol) (do (do (do b ob) ol) o2)) o1))
           (ensures eq (merge (do l ol) (do (do a ol) o1) (do (do (do (do b o) ob) ol) o2)) (do (merge (do l ol) (do a ol) (do (do (do (do b o) ob) ol) o2)) o1))
 
@@ -409,11 +497,13 @@ let inter_right_2op (l a b :concrete_st) (o1 o2 ob ol o:op_t)
                     eq (merge (do l ol) (do (do a ol) o1) (do (do (do b ob) ol) o2)) (do (merge (do l ol) (do a ol) (do (do (do b ob) ol) o2)) o1))
           (ensures eq (merge (do l ol) (do (do a ol) o1) (do (do (do (do b o) ob) ol) o2)) (do (merge (do l ol) (do a ol) (do (do (do (do b o) ob) ol) o2)) o1)) =
   let k = get_key o in
-  let ka = Alpha_t k in let kb = Beta_t k in
+  let ka = Alpha_t k in let kb = Beta_t k in let kc = Gamma_t k in
   if get_key o1 = k && get_key o2 = k && get_key ob = k && get_key ol = k && is_alpha_op o1 && is_alpha_op o2 && is_alpha_op ob && is_alpha_op ol && is_alpha_op o && (Fst_then_snd? (rc_a (get_op_a o2) (get_op_a o1)) || Either? (rc_a (get_op_a o2) (get_op_a o1))) && Fst_then_snd? (rc_a (get_op_a ob) (get_op_a ol)) && (Fst_then_snd? (rc_a (get_op_a o) (get_op_a ob)) || Snd_then_fst? (rc_a (get_op_a o) (get_op_a ob)) || Fst_then_snd? (rc_a (get_op_a o) (get_op_a ol))) then 
     inter_right_2op_a (sel l ka) (sel a ka) (sel b ka) (get_op_a o1) (get_op_a o2) (get_op_a ob) (get_op_a ol) (get_op_a o)
   else if get_key o1 = k && get_key o2 = k && get_key ob = k && get_key ol = k && is_beta_op o1 && is_beta_op o2 && is_beta_op ob && is_beta_op ol && is_beta_op o && (Fst_then_snd? (rc_b (get_op_b o2) (get_op_b o1)) || Either? (rc_b (get_op_b o2) (get_op_b o1))) && Fst_then_snd? (rc_b (get_op_b ob) (get_op_b ol)) && (Fst_then_snd? (rc_b (get_op_b o) (get_op_b ob)) || Snd_then_fst? (rc_b (get_op_b o) (get_op_b ob)) || Fst_then_snd? (rc_b (get_op_b o) (get_op_b ol))) then
     inter_right_2op_b (sel l kb) (sel a kb) (sel b kb) (get_op_b o1) (get_op_b o2) (get_op_b ob) (get_op_b ol) (get_op_b o)
+  else if get_key o1 = k && get_key o2 = k && get_key ob = k && get_key ol = k && is_gamma_op o1 && is_gamma_op o2 && is_gamma_op ob && is_gamma_op ol && is_gamma_op o && (Fst_then_snd? (rc_c (get_op_c o2) (get_op_c o1)) || Either? (rc_c (get_op_c o2) (get_op_c o1))) && Fst_then_snd? (rc_c (get_op_c ob) (get_op_c ol)) && (Fst_then_snd? (rc_c (get_op_c o) (get_op_c ob)) || Snd_then_fst? (rc_c (get_op_c o) (get_op_c ob)) || Fst_then_snd? (rc_c (get_op_c o) (get_op_c ol))) then
+    inter_right_2op_c (sel l kc) (sel a kc) (sel b kc) (get_op_c o1) (get_op_c o2) (get_op_c ob) (get_op_c ol) (get_op_c o)
   else if Either? (rc o2 o1) then inter_right_2op' l a b o1 o2 ob ol o
   else ()
 
@@ -432,6 +522,14 @@ val inter_left_2op_b (l a b :concrete_st_b) (o1 o2 ob ol o:op_b)
                     get_rid o <> get_rid ol /\
                     eq_b (merge_b (do_b l ol) (do_b (do_b (do_b a ob) ol) o1) (do_b (do_b b ol) o2)) (do_b (merge_b (do_b l ol) (do_b (do_b a ob) ol) (do_b (do_b b ol) o2)) o1))
           (ensures eq_b (merge_b (do_b l ol) (do_b (do_b (do_b (do_b a o) ob) ol) o1) (do_b (do_b b ol) o2)) (do_b (merge_b (do_b l ol) (do_b (do_b (do_b a o) ob) ol) (do_b (do_b b ol) o2)) o1))
+
+val inter_left_2op_c (l a b :concrete_st_c) (o1 o2 ob ol o:op_c)
+  : Lemma (requires (Fst_then_snd? (rc_c o2 o1) \/ Either? (rc_c o2 o1)) /\ get_rid o1 <> get_rid o2 /\ Fst_then_snd? (rc_c ob ol) /\ get_rid ob <> get_rid ol /\
+                    (~ (Either? (rc_c o ob)) \/ Fst_then_snd? (rc_c o ol)) /\
+                    distinct_ops o1 o2 /\ distinct_ops o1 ob /\ distinct_ops o1 ol /\ distinct_ops o1 o /\ distinct_ops o2 ob /\ distinct_ops o2 ol /\ distinct_ops o2 o /\ distinct_ops ob ol /\ distinct_ops ob o /\ distinct_ops ol o /\
+                    get_rid o <> get_rid ol /\
+                    eq_c (merge_c (do_c l ol) (do_c (do_c (do_c a ob) ol) o1) (do_c (do_c b ol) o2)) (do_c (merge_c (do_c l ol) (do_c (do_c a ob) ol) (do_c (do_c b ol) o2)) o1))
+          (ensures eq_c (merge_c (do_c l ol) (do_c (do_c (do_c (do_c a o) ob) ol) o1) (do_c (do_c b ol) o2)) (do_c (merge_c (do_c l ol) (do_c (do_c (do_c a o) ob) ol) (do_c (do_c b ol) o2)) o1))
           
 val inter_left_2op' (l a b :concrete_st) (o1 o2 ob ol o:op_t)
   : Lemma (requires Either? (rc o2 o1) /\ get_rid o1 <> get_rid o2 /\ Fst_then_snd? (rc ob ol) /\ get_rid ob <> get_rid ol /\
@@ -439,7 +537,8 @@ val inter_left_2op' (l a b :concrete_st) (o1 o2 ob ol o:op_t)
                     get_rid o <> get_rid ol /\
                     ~ (get_key o1 = get_key o && get_key o2 = get_key o /\ get_key ob = get_key o /\ get_key ol = get_key o /\
                        is_alpha_op o1 /\ is_alpha_op o2 /\ is_alpha_op ob /\ is_alpha_op ol /\ is_alpha_op o /\ (Fst_then_snd? (rc_a (get_op_a o2) (get_op_a o1)) \/ Either? (rc_a (get_op_a o2) (get_op_a o1))) /\ Fst_then_snd? (rc_a (get_op_a ob) (get_op_a ol)) /\ (Fst_then_snd? (rc_a (get_op_a o) (get_op_a ob)) \/ Snd_then_fst? (rc_a (get_op_a o) (get_op_a ob)) \/ Fst_then_snd? (rc_a (get_op_a o) (get_op_a ol))) /\
-                       is_beta_op o1 /\ is_beta_op o2 /\ is_beta_op ob /\ is_beta_op ol /\ is_beta_op o /\ (Fst_then_snd? (rc_b (get_op_b o2) (get_op_b o1)) \/ Either? (rc_b (get_op_b o2) (get_op_b o1))) /\ Fst_then_snd? (rc_b (get_op_b ob) (get_op_b ol)) /\ (Fst_then_snd? (rc_b (get_op_b o) (get_op_b ob)) \/ Snd_then_fst? (rc_b (get_op_b o) (get_op_b ob)) \/ Fst_then_snd? (rc_b (get_op_b o) (get_op_b ol)))) /\
+                       is_beta_op o1 /\ is_beta_op o2 /\ is_beta_op ob /\ is_beta_op ol /\ is_beta_op o /\ (Fst_then_snd? (rc_b (get_op_b o2) (get_op_b o1)) \/ Either? (rc_b (get_op_b o2) (get_op_b o1))) /\ Fst_then_snd? (rc_b (get_op_b ob) (get_op_b ol)) /\ (Fst_then_snd? (rc_b (get_op_b o) (get_op_b ob)) \/ Snd_then_fst? (rc_b (get_op_b o) (get_op_b ob)) \/ Fst_then_snd? (rc_b (get_op_b o) (get_op_b ol))) /\
+                       is_gamma_op o1 /\ is_gamma_op o2 /\ is_gamma_op ob /\ is_gamma_op ol /\ is_gamma_op o /\ (Fst_then_snd? (rc_c (get_op_c o2) (get_op_c o1)) \/ Either? (rc_c (get_op_c o2) (get_op_c o1))) /\ Fst_then_snd? (rc_c (get_op_c ob) (get_op_c ol)) /\ (Fst_then_snd? (rc_c (get_op_c o) (get_op_c ob)) \/ Snd_then_fst? (rc_c (get_op_c o) (get_op_c ob)) \/ Fst_then_snd? (rc_c (get_op_c o) (get_op_c ol)))) /\
                     eq (merge (do l ol) (do (do (do a ob) ol) o1) (do (do b ol) o2)) (do (merge (do l ol) (do (do a ob) ol) (do (do b ol) o2)) o1))
           (ensures eq (merge (do l ol) (do (do (do (do a o) ob) ol) o1) (do (do b ol) o2)) (do (merge (do l ol) (do (do (do a o) ob) ol) (do (do b ol) o2)) o1))
 
@@ -452,11 +551,13 @@ let inter_left_2op (l a b :concrete_st) (o1 o2 ob ol o:op_t)
                     eq (merge (do l ol) (do (do (do a ob) ol) o1) (do (do b ol) o2)) (do (merge (do l ol) (do (do a ob) ol) (do (do b ol) o2)) o1))
           (ensures eq (merge (do l ol) (do (do (do (do a o) ob) ol) o1) (do (do b ol) o2)) (do (merge (do l ol) (do (do (do a o) ob) ol) (do (do b ol) o2)) o1)) =
   let k = get_key o in
-  let ka = Alpha_t k in let kb = Beta_t k in
+  let ka = Alpha_t k in let kb = Beta_t k in let kc = Gamma_t k in
   if get_key o1 = k && get_key o2 = k && get_key ob = k && get_key ol = k && is_alpha_op o1 && is_alpha_op o2 && is_alpha_op ob && is_alpha_op ol && is_alpha_op o && (Fst_then_snd? (rc_a (get_op_a o2) (get_op_a o1)) || Either? (rc_a (get_op_a o2) (get_op_a o1))) && Fst_then_snd? (rc_a (get_op_a ob) (get_op_a ol)) && (Fst_then_snd? (rc_a (get_op_a o) (get_op_a ob)) || Snd_then_fst? (rc_a (get_op_a o) (get_op_a ob)) || Fst_then_snd? (rc_a (get_op_a o) (get_op_a ol))) then 
     inter_left_2op_a (sel l ka) (sel a ka) (sel b ka) (get_op_a o1) (get_op_a o2) (get_op_a ob) (get_op_a ol) (get_op_a o)
   else if get_key o1 = k && get_key o2 = k && get_key ob = k && get_key ol = k && is_beta_op o1 && is_beta_op o2 && is_beta_op ob && is_beta_op ol && is_beta_op o && (Fst_then_snd? (rc_b (get_op_b o2) (get_op_b o1)) || Either? (rc_b (get_op_b o2) (get_op_b o1))) && Fst_then_snd? (rc_b (get_op_b ob) (get_op_b ol)) && (Fst_then_snd? (rc_b (get_op_b o) (get_op_b ob)) || Snd_then_fst? (rc_b (get_op_b o) (get_op_b ob)) || Fst_then_snd? (rc_b (get_op_b o) (get_op_b ol))) then
     inter_left_2op_b (sel l kb) (sel a kb) (sel b kb) (get_op_b o1) (get_op_b o2) (get_op_b ob) (get_op_b ol) (get_op_b o)
+  else if get_key o1 = k && get_key o2 = k && get_key ob = k && get_key ol = k && is_gamma_op o1 && is_gamma_op o2 && is_gamma_op ob && is_gamma_op ol && is_gamma_op o && (Fst_then_snd? (rc_c (get_op_c o2) (get_op_c o1)) || Either? (rc_c (get_op_c o2) (get_op_c o1))) && Fst_then_snd? (rc_c (get_op_c ob) (get_op_c ol)) && (Fst_then_snd? (rc_c (get_op_c o) (get_op_c ob)) || Snd_then_fst? (rc_c (get_op_c o) (get_op_c ob)) || Fst_then_snd? (rc_c (get_op_c o) (get_op_c ol))) then
+    inter_left_2op_c (sel l kc) (sel a kc) (sel b kc) (get_op_c o1) (get_op_c o2) (get_op_c ob) (get_op_c ol) (get_op_c o)
   else if Either? (rc o2 o1) then inter_left_2op' l a b o1 o2 ob ol o
   else ()
 
@@ -472,17 +573,25 @@ val ind_right_2op_b (l a b:concrete_st_b) (o1 o2 o2':op_b)
                     eq_b (merge_b l (do_b a o1) (do_b b o2)) (do_b (merge_b l a (do_b b o2)) o1))
           (ensures eq_b (merge_b l (do_b a o1) (do_b (do_b b o2') o2)) (do_b (merge_b l a (do_b (do_b b o2') o2)) o1))
 
+val ind_right_2op_c (l a b:concrete_st_c) (o1 o2 o2':op_c)
+  : Lemma (requires Fst_then_snd? (rc_c o2 o1) /\ get_rid o1 <> get_rid o2 /\
+                    distinct_ops o1 o2 /\ distinct_ops o1 o2' /\ distinct_ops o2 o2' /\
+                    eq_c (merge_c l (do_c a o1) (do_c b o2)) (do_c (merge_c l a (do_c b o2)) o1))
+          (ensures eq_c (merge_c l (do_c a o1) (do_c (do_c b o2') o2)) (do_c (merge_c l a (do_c (do_c b o2') o2)) o1))
+          
 let ind_right_2op (l a b:concrete_st) (o1 o2 o2':op_t)
   : Lemma (requires Fst_then_snd? (rc o2 o1) /\ get_rid o1 <> get_rid o2 /\
                     distinct_ops o1 o2 /\ distinct_ops o1 o2' /\ distinct_ops o2 o2' /\
                     eq (merge l (do a o1) (do b o2)) (do (merge l a (do b o2)) o1))
           (ensures eq (merge l (do a o1) (do (do b o2') o2)) (do (merge l a (do (do b o2') o2)) o1)) =
   let k = get_key o2' in
-  let ka = Alpha_t k in let kb = Beta_t k in
+  let ka = Alpha_t k in let kb = Beta_t k in let kc = Gamma_t k in
   if get_key o1 = k && get_key o2 = k && is_alpha_op o1 && is_alpha_op o2 && is_alpha_op o2' && Fst_then_snd? (rc_a (get_op_a o2) (get_op_a o1)) then
       ind_right_2op_a (sel l ka) (sel a ka) (sel b ka) (get_op_a o1) (get_op_a o2) (get_op_a o2')
   else if get_key o1 = k && get_key o2 = k && is_beta_op o1 && is_beta_op o2 && is_beta_op o2' && Fst_then_snd? (rc_b (get_op_b o2) (get_op_b o1)) then
       ind_right_2op_b (sel l kb) (sel a kb) (sel b kb) (get_op_b o1) (get_op_b o2) (get_op_b o2')
+  else if get_key o1 = k && get_key o2 = k && is_gamma_op o1 && is_gamma_op o2 && is_gamma_op o2' && Fst_then_snd? (rc_c (get_op_c o2) (get_op_c o1)) then
+      ind_right_2op_c (sel l kc) (sel a kc) (sel b kc) (get_op_c o1) (get_op_c o2) (get_op_c o2')
   else ()
 
 val ind_left_2op_a (l a b:concrete_st_a) (o1 o2 o1':op_a)
@@ -497,17 +606,25 @@ val ind_left_2op_b (l a b:concrete_st_b) (o1 o2 o1':op_b)
                     eq_b (merge_b l (do_b a o1) (do_b b o2)) (do_b (merge_b l a (do_b b o2)) o1))
           (ensures eq_b (merge_b l (do_b (do_b a o1') o1) (do_b b o2)) (do_b (merge_b l (do_b a o1') (do_b b o2)) o1))
 
+val ind_left_2op_c (l a b:concrete_st_c) (o1 o2 o1':op_c)
+  : Lemma (requires Fst_then_snd? (rc_c o2 o1) /\ get_rid o1 <> get_rid o2 /\
+                    distinct_ops o1 o2 /\ distinct_ops o1 o1' /\ distinct_ops o2 o1' /\
+                    eq_c (merge_c l (do_c a o1) (do_c b o2)) (do_c (merge_c l a (do_c b o2)) o1))
+          (ensures eq_c (merge_c l (do_c (do_c a o1') o1) (do_c b o2)) (do_c (merge_c l (do_c a o1') (do_c b o2)) o1))
+          
 let ind_left_2op (l a b:concrete_st) (o1 o2 o1':op_t)
   : Lemma (requires Fst_then_snd? (rc o2 o1) /\ get_rid o1 <> get_rid o2 /\
                     distinct_ops o1 o2 /\ distinct_ops o1 o1' /\ distinct_ops o2 o1' /\
                     eq (merge l (do a o1) (do b o2)) (do (merge l a (do b o2)) o1))
           (ensures eq (merge l (do (do a o1') o1) (do b o2)) (do (merge l (do a o1') (do b o2)) o1)) =
   let k = get_key o1' in
-  let ka = Alpha_t k in let kb = Beta_t k in
+  let ka = Alpha_t k in let kb = Beta_t k in let kc = Gamma_t k in
   if get_key o1 = k && get_key o2 = k && is_alpha_op o1 && is_alpha_op o2 && is_alpha_op o1' && Fst_then_snd? (rc_a (get_op_a o2) (get_op_a o1)) then
       ind_left_2op_a (sel l ka) (sel a ka) (sel b ka) (get_op_a o1) (get_op_a o2) (get_op_a o1')
   else if get_key o1 = k && get_key o2 = k && is_beta_op o1 && is_beta_op o2 && is_beta_op o1' && Fst_then_snd? (rc_b (get_op_b o2) (get_op_b o1)) then
       ind_left_2op_b (sel l kb) (sel a kb) (sel b kb) (get_op_b o1) (get_op_b o2) (get_op_b o1')
+  else if get_key o1 = k && get_key o2 = k && is_gamma_op o1 && is_gamma_op o2 && is_gamma_op o1' && Fst_then_snd? (rc_c (get_op_c o2) (get_op_c o1)) then
+      ind_left_2op_c (sel l kc) (sel a kc) (sel b kc) (get_op_c o1) (get_op_c o2) (get_op_c o1')
   else ()
 
 (*One OP*)
@@ -518,10 +635,14 @@ val base_1op_a (o1:op_a)
 val base_1op_b (o1:op_b) 
   : Lemma (ensures eq_b (merge_b init_st_b (do_b init_st_b o1) init_st_b) (do_b (merge_b init_st_b init_st_b init_st_b) o1))
 
+val base_1op_c (o1:op_c) 
+  : Lemma (ensures eq_c (merge_c init_st_c (do_c init_st_c o1) init_st_c) (do_c (merge_c init_st_c init_st_c init_st_c) o1))
+  
 let base_1op (o1:op_t) (t:kt)
   : Lemma (ensures eq (merge (init_st t) (do (init_st t) o1) (init_st t)) (do (merge (init_st t) (init_st t) (init_st t)) o1)) =
   if is_alpha_op o1 then base_1op_a (get_op_a o1)
   else if is_beta_op o1 then base_1op_b (get_op_b o1)
+  else if is_gamma_op o1 then base_1op_c (get_op_c o1)
   else ()
 
 val ind_lca_1op_a (l:concrete_st_a) (o1 ol:op_a)
@@ -534,16 +655,23 @@ val ind_lca_1op_b (l:concrete_st_b) (o1 ol:op_b)
                     eq_b (merge_b l (do_b l o1) l) (do_b (merge_b l l l) o1))
           (ensures eq_b (merge_b (do_b l ol) (do_b (do_b l ol) o1) (do_b l ol)) (do_b (merge_b (do_b l ol) (do_b l ol) (do_b l ol)) o1))
 
+val ind_lca_1op_c (l:concrete_st_c) (o1 ol:op_c)
+  : Lemma (requires distinct_ops o1 ol /\ 
+                    eq_c (merge_c l (do_c l o1) l) (do_c (merge_c l l l) o1))
+          (ensures eq_c (merge_c (do_c l ol) (do_c (do_c l ol) o1) (do_c l ol)) (do_c (merge_c (do_c l ol) (do_c l ol) (do_c l ol)) o1))
+
 let ind_lca_1op (l:concrete_st) (o1 ol:op_t)
   : Lemma (requires distinct_ops o1 ol /\
                     eq (merge l (do l o1) l) (do (merge l l l) o1))
           (ensures eq (merge (do l ol) (do (do l ol) o1) (do l ol)) (do (merge (do l ol) (do l ol) (do l ol)) o1)) =
   let k = get_key ol in
-  let ka = Alpha_t k in let kb = Beta_t k in
+  let ka = Alpha_t k in let kb = Beta_t k in let kc = Gamma_t k in
   if get_key o1 = k && is_alpha_op o1 && is_alpha_op ol then
       ind_lca_1op_a (sel l ka) (get_op_a o1) (get_op_a ol)
   else if get_key o1 = k && is_beta_op o1 && is_beta_op ol then
       ind_lca_1op_b (sel l kb) (get_op_b o1) (get_op_b ol)
+  else if get_key o1 = k && is_gamma_op o1 && is_gamma_op ol then
+      ind_lca_1op_c (sel l kc) (get_op_c o1) (get_op_c ol)
   else ()
 
 val inter_right_base_1op_a (l a b :concrete_st_a) (o1 ob ol:op_a)
@@ -559,7 +687,14 @@ val inter_right_base_1op_b (l a b :concrete_st_b) (o1 ob ol:op_b)
                     (Fst_then_snd? (rc_b ob o1) ==> eq_b (merge_b l (do_b a o1) (do_b b ob)) (do_b (merge_b l a (do_b b ob)) o1)) /\ //from app.fsti
                     eq_b (merge_b (do_b l ol) (do_b (do_b a ol) o1) (do_b b ol)) (do_b (merge_b (do_b l ol) (do_b a ol) (do_b b ol)) o1))
           (ensures eq_b (merge_b (do_b l ol) (do_b (do_b a ol) o1) (do_b (do_b b ob) ol)) (do_b (merge_b (do_b l ol) (do_b a ol) (do_b (do_b b ob) ol)) o1))
-          
+
+val inter_right_base_1op_c (l a b :concrete_st_c) (o1 ob ol:op_c)
+  : Lemma (requires Fst_then_snd? (rc_c ob ol) /\ get_rid ob <> get_rid ol /\
+                    distinct_ops o1 ob /\ distinct_ops o1 ol /\ distinct_ops ob ol /\
+                    (Fst_then_snd? (rc_c ob o1) ==> eq_c (merge_c l (do_c a o1) (do_c b ob)) (do_c (merge_c l a (do_c b ob)) o1)) /\ //from app.fsti
+                    eq_c (merge_c (do_c l ol) (do_c (do_c a ol) o1) (do_c b ol)) (do_c (merge_c (do_c l ol) (do_c a ol) (do_c b ol)) o1))
+          (ensures eq_c (merge_c (do_c l ol) (do_c (do_c a ol) o1) (do_c (do_c b ob) ol)) (do_c (merge_c (do_c l ol) (do_c a ol) (do_c (do_c b ob) ol)) o1))
+
 let inter_right_base_1op (l a b :concrete_st) (o1 ob ol:op_t)
   : Lemma (requires Fst_then_snd? (rc ob ol) /\ get_rid ob <> get_rid ol /\
                     distinct_ops o1 ob /\ distinct_ops o1 ol /\ distinct_ops ob ol /\
@@ -567,11 +702,13 @@ let inter_right_base_1op (l a b :concrete_st) (o1 ob ol:op_t)
                     eq (merge (do l ol) (do (do a ol) o1) (do b ol)) (do (merge (do l ol) (do a ol) (do b ol)) o1))
           (ensures eq (merge (do l ol) (do (do a ol) o1) (do (do b ob) ol)) (do (merge (do l ol) (do a ol) (do (do b ob) ol)) o1)) =
   let k = get_key ol in
-  let ka = Alpha_t k in let kb = Beta_t k in
+  let ka = Alpha_t k in let kb = Beta_t k in let kc = Gamma_t k in
   if get_key o1 = k && get_key ob = k && is_alpha_op o1 && is_alpha_op ob && is_alpha_op ol && Fst_then_snd? (rc_a (get_op_a ob) (get_op_a ol)) then
       inter_right_base_1op_a (sel l ka) (sel a ka) (sel b ka) (get_op_a o1) (get_op_a ob) (get_op_a ol)
   else if get_key o1 = k && get_key ob = k && is_beta_op o1 && is_beta_op ob && is_beta_op ol && Fst_then_snd? (rc_b (get_op_b ob) (get_op_b ol)) then
       inter_right_base_1op_b (sel l kb) (sel a kb) (sel b kb) (get_op_b o1) (get_op_b ob) (get_op_b ol)
+  else if get_key o1 = k && get_key ob = k && is_gamma_op o1 && is_gamma_op ob && is_gamma_op ol && Fst_then_snd? (rc_c (get_op_c ob) (get_op_c ol)) then
+      inter_right_base_1op_c (sel l kc) (sel a kc) (sel b kc) (get_op_c o1) (get_op_c ob) (get_op_c ol)
   else ()
 
 val inter_left_base_1op_a (l a b :concrete_st_a) (o1 ob ol:op_a)
@@ -585,18 +722,26 @@ val inter_left_base_1op_b (l a b :concrete_st_b) (o1 ob ol:op_b)
                     distinct_ops o1 ob /\ distinct_ops o1 ol /\ distinct_ops ob ol /\
                     eq_b (merge_b (do_b l ol) (do_b (do_b a ol) o1) (do_b b ol)) (do_b (merge_b (do_b l ol) (do_b a ol) (do_b b ol)) o1))
           (ensures eq_b (merge_b (do_b l ol) (do_b (do_b (do_b a ob) ol) o1) (do_b b ol)) (do_b (merge_b (do_b l ol) (do_b (do_b a ob) ol) (do_b b ol)) o1))
-          
+
+val inter_left_base_1op_c (l a b :concrete_st_c) (o1 ob ol:op_c)
+  : Lemma (requires Fst_then_snd? (rc_c ob ol) /\ get_rid ob <> get_rid ol /\
+                    distinct_ops o1 ob /\ distinct_ops o1 ol /\ distinct_ops ob ol /\
+                    eq_c (merge_c (do_c l ol) (do_c (do_c a ol) o1) (do_c b ol)) (do_c (merge_c (do_c l ol) (do_c a ol) (do_c b ol)) o1))
+          (ensures eq_c (merge_c (do_c l ol) (do_c (do_c (do_c a ob) ol) o1) (do_c b ol)) (do_c (merge_c (do_c l ol) (do_c (do_c a ob) ol) (do_c b ol)) o1))
+
 let inter_left_base_1op (l a b:concrete_st) (o1 ob ol:op_t)
   : Lemma (requires Fst_then_snd? (rc ob ol) /\ get_rid ob <> get_rid ol /\
                     distinct_ops o1 ob /\ distinct_ops o1 ol /\ distinct_ops ob ol /\
                     eq (merge (do l ol) (do (do a ol) o1) (do b ol)) (do (merge (do l ol) (do a ol) (do b ol)) o1))
           (ensures eq (merge (do l ol) (do (do (do a ob) ol) o1) (do b ol)) (do (merge (do l ol) (do (do a ob) ol) (do b ol)) o1)) =
   let k = get_key ol in
-  let ka = Alpha_t k in let kb = Beta_t k in
+  let ka = Alpha_t k in let kb = Beta_t k in let kc = Gamma_t k in
   if get_key o1 = k && get_key ob = k && is_alpha_op o1 && is_alpha_op ob && is_alpha_op ol && Fst_then_snd? (rc_a (get_op_a ob) (get_op_a ol)) then
       inter_left_base_1op_a (sel l ka) (sel a ka) (sel b ka) (get_op_a o1) (get_op_a ob) (get_op_a ol)
   else if get_key o1 = k && get_key ob = k && is_beta_op o1 && is_beta_op ob && is_beta_op ol && Fst_then_snd? (rc_b (get_op_b ob) (get_op_b ol)) then
       inter_left_base_1op_b (sel l kb) (sel a kb) (sel b kb) (get_op_b o1) (get_op_b ob) (get_op_b ol)
+  else if get_key o1 = k && get_key ob = k && is_gamma_op o1 && is_gamma_op ob && is_gamma_op ol && Fst_then_snd? (rc_c (get_op_c ob) (get_op_c ol)) then
+      inter_left_base_1op_c (sel l kc) (sel a kc) (sel b kc) (get_op_c o1) (get_op_c ob) (get_op_c ol)
   else ()
 
 val inter_right_1op_a (l a b :concrete_st_a) (o1 ob ol o:op_a)
@@ -614,6 +759,14 @@ val inter_right_1op_b (l a b :concrete_st_b) (o1 ob ol o:op_b)
                     get_rid o <> get_rid ol /\
                     eq_b (merge_b (do_b l ol) (do_b (do_b a ol) o1) (do_b (do_b b ob) ol)) (do_b (merge_b (do_b l ol) (do_b a ol) (do_b (do_b b ob) ol)) o1))
           (ensures eq_b (merge_b (do_b l ol) (do_b (do_b a ol) o1) (do_b (do_b (do_b b o) ob) ol)) (do_b (merge_b (do_b l ol) (do_b a ol) (do_b (do_b (do_b b o) ob) ol)) o1))
+
+val inter_right_1op_c (l a b :concrete_st_c) (o1 ob ol o:op_c)
+  : Lemma (requires Fst_then_snd? (rc_c ob ol) /\ get_rid ob <> get_rid ol /\
+                    (~ (Either? (rc_c o ob)) \/ Fst_then_snd? (rc_c o ol)) /\
+                    distinct_ops o1 ob /\ distinct_ops o1 ol /\ distinct_ops o1 o /\ distinct_ops ob ol /\ distinct_ops ob o /\ distinct_ops ol o /\
+                    get_rid o <> get_rid ol /\
+                    eq_c (merge_c (do_c l ol) (do_c (do_c a ol) o1) (do_c (do_c b ob) ol)) (do_c (merge_c (do_c l ol) (do_c a ol) (do_c (do_c b ob) ol)) o1))
+          (ensures eq_c (merge_c (do_c l ol) (do_c (do_c a ol) o1) (do_c (do_c (do_c b o) ob) ol)) (do_c (merge_c (do_c l ol) (do_c a ol) (do_c (do_c (do_c b o) ob) ol)) o1))
           
 let inter_right_1op (l a b:concrete_st) (o1 ob ol o:op_t) 
   : Lemma (requires Fst_then_snd? (rc ob ol) /\ get_rid ob <> get_rid ol /\
@@ -623,11 +776,13 @@ let inter_right_1op (l a b:concrete_st) (o1 ob ol o:op_t)
                     eq (merge (do l ol) (do (do a ol) o1) (do (do b ob) ol)) (do (merge (do l ol) (do a ol) (do (do b ob) ol)) o1))
           (ensures eq (merge (do l ol) (do (do a ol) o1) (do (do (do b o) ob) ol)) (do (merge (do l ol) (do a ol) (do (do (do b o) ob) ol)) o1)) =
   let k = get_key o in
-  let ka = Alpha_t k in let kb = Beta_t k in
+  let ka = Alpha_t k in let kb = Beta_t k in let kc = Gamma_t k in
   if get_key o1 = k && get_key ob = k && get_key ol = k && is_alpha_op o1 && is_alpha_op ob && is_alpha_op ol && is_alpha_op o && Fst_then_snd? (rc_a (get_op_a ob) (get_op_a ol)) && (Fst_then_snd? (rc_a (get_op_a o) (get_op_a ob)) || Snd_then_fst? (rc_a (get_op_a o) (get_op_a ob)) || Fst_then_snd? (rc_a (get_op_a o) (get_op_a ol))) then 
     inter_right_1op_a (sel l ka) (sel a ka) (sel b ka) (get_op_a o1) (get_op_a ob) (get_op_a ol) (get_op_a o)
   else if get_key o1 = k && get_key ob = k && get_key ol = k && is_beta_op o1 && is_beta_op ob && is_beta_op ol && is_beta_op o && Fst_then_snd? (rc_b (get_op_b ob) (get_op_b ol)) && (Fst_then_snd? (rc_b (get_op_b o) (get_op_b ob)) || Snd_then_fst? (rc_b (get_op_b o) (get_op_b ob)) || Fst_then_snd? (rc_b (get_op_b o) (get_op_b ol))) then
     inter_right_1op_b (sel l kb) (sel a kb) (sel b kb) (get_op_b o1) (get_op_b ob) (get_op_b ol) (get_op_b o)
+  else if get_key o1 = k && get_key ob = k && get_key ol = k && is_gamma_op o1 && is_gamma_op ob && is_gamma_op ol && is_gamma_op o && Fst_then_snd? (rc_c (get_op_c ob) (get_op_c ol)) && (Fst_then_snd? (rc_c (get_op_c o) (get_op_c ob)) || Snd_then_fst? (rc_c (get_op_c o) (get_op_c ob)) || Fst_then_snd? (rc_c (get_op_c o) (get_op_c ol))) then
+    inter_right_1op_c (sel l kc) (sel a kc) (sel b kc) (get_op_c o1) (get_op_c ob) (get_op_c ol) (get_op_c o)
   else ()
 
 val inter_left_1op_a (l a b :concrete_st_a) (o1 ob ol o:op_a)
@@ -645,6 +800,14 @@ val inter_left_1op_b (l a b :concrete_st_b) (o1 ob ol o:op_b)
                     get_rid o <> get_rid ol /\
                     eq_b (merge_b (do_b l ol) (do_b (do_b (do_b a ob) ol) o1) (do_b b ol)) (do_b (merge_b (do_b l ol) (do_b (do_b a ob) ol) (do_b b ol)) o1))
           (ensures eq_b (merge_b (do_b l ol) (do_b (do_b (do_b (do_b a o) ob) ol) o1) (do_b b ol)) (do_b (merge_b (do_b l ol) (do_b (do_b (do_b a o) ob) ol) (do_b b ol)) o1))
+
+val inter_left_1op_c (l a b :concrete_st_c) (o1 ob ol o:op_c)
+  : Lemma (requires Fst_then_snd? (rc_c ob ol) /\ get_rid ob <> get_rid ol /\
+                    (~ (Either? (rc_c o ob)) \/ Fst_then_snd? (rc_c o ol)) /\
+                    distinct_ops o1 ob /\ distinct_ops o1 ol /\ distinct_ops o1 o /\ distinct_ops ob ol /\ distinct_ops ob o /\ distinct_ops ol o /\
+                    get_rid o <> get_rid ol /\
+                    eq_c (merge_c (do_c l ol) (do_c (do_c (do_c a ob) ol) o1) (do_c b ol)) (do_c (merge_c (do_c l ol) (do_c (do_c a ob) ol) (do_c b ol)) o1))
+          (ensures eq_c (merge_c (do_c l ol) (do_c (do_c (do_c (do_c a o) ob) ol) o1) (do_c b ol)) (do_c (merge_c (do_c l ol) (do_c (do_c (do_c a o) ob) ol) (do_c b ol)) o1))
           
 let inter_left_1op (l a b :concrete_st) (o1 ob ol o:op_t)
   : Lemma (requires Fst_then_snd? (rc ob ol) /\ get_rid ob <> get_rid ol /\
@@ -654,11 +817,13 @@ let inter_left_1op (l a b :concrete_st) (o1 ob ol o:op_t)
                     eq (merge (do l ol) (do (do (do a ob) ol) o1) (do b ol)) (do (merge (do l ol) (do (do a ob) ol) (do b ol)) o1))
           (ensures eq (merge (do l ol) (do (do (do (do a o) ob) ol) o1) (do b ol)) (do (merge (do l ol) (do (do (do a o) ob) ol) (do b ol)) o1)) =
   let k = get_key o in
-  let ka = Alpha_t k in let kb = Beta_t k in
+  let ka = Alpha_t k in let kb = Beta_t k in let kc = Gamma_t k in
   if get_key o1 = k && get_key ob = k && get_key ol = k && is_alpha_op o1 && is_alpha_op ob && is_alpha_op ol && is_alpha_op o && Fst_then_snd? (rc_a (get_op_a ob) (get_op_a ol)) && (Fst_then_snd? (rc_a (get_op_a o) (get_op_a ob)) || Snd_then_fst? (rc_a (get_op_a o) (get_op_a ob)) || Fst_then_snd? (rc_a (get_op_a o) (get_op_a ol))) then 
     inter_left_1op_a (sel l ka) (sel a ka) (sel b ka) (get_op_a o1) (get_op_a ob) (get_op_a ol) (get_op_a o)
   else if get_key o1 = k && get_key ob = k && get_key ol = k && is_beta_op o1 && is_beta_op ob && is_beta_op ol && is_beta_op o && Fst_then_snd? (rc_b (get_op_b ob) (get_op_b ol)) && (Fst_then_snd? (rc_b (get_op_b o) (get_op_b ob)) || Snd_then_fst? (rc_b (get_op_b o) (get_op_b ob)) || Fst_then_snd? (rc_b (get_op_b o) (get_op_b ol))) then
     inter_left_1op_b (sel l kb) (sel a kb) (sel b kb) (get_op_b o1) (get_op_b ob) (get_op_b ol) (get_op_b o)
+  else if get_key o1 = k && get_key ob = k && get_key ol = k && is_gamma_op o1 && is_gamma_op ob && is_gamma_op ol && is_gamma_op o && Fst_then_snd? (rc_c (get_op_c ob) (get_op_c ol)) && (Fst_then_snd? (rc_c (get_op_c o) (get_op_c ob)) || Snd_then_fst? (rc_c (get_op_c o) (get_op_c ob)) || Fst_then_snd? (rc_c (get_op_c o) (get_op_c ol))) then
+    inter_left_1op_c (sel l kc) (sel a kc) (sel b kc) (get_op_c o1) (get_op_c ob) (get_op_c ol) (get_op_c o)
   else ()
 
 val ind_right_1op_a (l a b:concrete_st_a) (o2 o2' ol:op_a)
@@ -670,6 +835,11 @@ val ind_right_1op_b (l a b:concrete_st_b) (o2 o2' ol:op_b)
   : Lemma (requires distinct_ops o2 o2' /\ distinct_ops o2 ol /\ distinct_ops o2' ol /\
                     eq_b (merge_b (do_b l ol) (do_b a ol) (do_b b o2)) (do_b (merge_b (do_b l ol) (do_b a ol) b) o2))
           (ensures eq_b (merge_b (do_b l ol) (do_b a ol) (do_b (do_b b o2') o2)) (do_b (merge_b (do_b l ol) (do_b a ol) (do_b b o2')) o2))
+
+val ind_right_1op_c (l a b:concrete_st_c) (o2 o2' ol:op_c)
+  : Lemma (requires distinct_ops o2 o2' /\ distinct_ops o2 ol /\ distinct_ops o2' ol /\
+                    eq_c (merge_c (do_c l ol) (do_c a ol) (do_c b o2)) (do_c (merge_c (do_c l ol) (do_c a ol) b) o2))
+          (ensures eq_c (merge_c (do_c l ol) (do_c a ol) (do_c (do_c b o2') o2)) (do_c (merge_c (do_c l ol) (do_c a ol) (do_c b o2')) o2))
 
 val ind_right_1op' (l a b:concrete_st) (o2 o2' ol:op_t)
   : Lemma (requires distinct_ops o2 o2' /\ distinct_ops o2 ol /\ distinct_ops o2' ol /\
@@ -684,11 +854,13 @@ let ind_right_1op (l a b:concrete_st) (o2 o2' ol:op_t)
                     eq (merge (do l ol) (do a ol) (do b o2)) (do (merge (do l ol) (do a ol) b) o2))
           (ensures eq (merge (do l ol) (do a ol) (do (do b o2') o2)) (do (merge (do l ol) (do a ol) (do b o2')) o2)) =
   let k = get_key ol in
-  let ka = Alpha_t k in let kb = Beta_t k in
+  let ka = Alpha_t k in let kb = Beta_t k in let kc = Gamma_t k in
   if get_key o2 = k && get_key o2' = k && is_alpha_op o2 && is_alpha_op o2' && is_alpha_op ol then
       ind_right_1op_a (sel l ka) (sel a ka) (sel b ka) (get_op_a o2) (get_op_a o2') (get_op_a ol)
   else if get_key o2 = k && get_key o2' = k && is_beta_op o2 && is_beta_op o2' && is_beta_op ol then
       ind_right_1op_b (sel l kb) (sel a kb) (sel b kb) (get_op_b o2) (get_op_b o2') (get_op_b ol)
+  else if get_key o2 = k && get_key o2' = k && is_gamma_op o2 && is_gamma_op o2' && is_gamma_op ol then
+      ind_right_1op_c (sel l kc) (sel a kc) (sel b kc) (get_op_c o2) (get_op_c o2') (get_op_c ol)
   else ind_right_1op' l a b o2 o2' ol
 
 val ind_left_1op_a (l a b:concrete_st_a) (o1 o1' ol:op_a)
@@ -701,6 +873,11 @@ val ind_left_1op_b (l a b:concrete_st_b) (o1 o1' ol:op_b)
                     eq_b (merge_b (do_b l ol) (do_b a o1) (do_b b ol)) (do_b (merge_b (do_b l ol) a (do_b b ol)) o1))
           (ensures eq_b (merge_b (do_b l ol) (do_b (do_b a o1') o1) (do_b b ol)) (do_b (merge_b (do_b l ol) (do_b a o1') (do_b b ol)) o1))
 
+val ind_left_1op_c (l a b:concrete_st_c) (o1 o1' ol:op_c)
+  : Lemma (requires distinct_ops o1 o1' /\ distinct_ops o1 ol /\ distinct_ops o1' ol /\
+                    eq_c (merge_c (do_c l ol) (do_c a o1) (do_c b ol)) (do_c (merge_c (do_c l ol) a (do_c b ol)) o1))
+          (ensures eq_c (merge_c (do_c l ol) (do_c (do_c a o1') o1) (do_c b ol)) (do_c (merge_c (do_c l ol) (do_c a o1') (do_c b ol)) o1))
+          
 val ind_left_1op' (l a b:concrete_st) (o1 o1' ol:op_t)
   : Lemma (requires distinct_ops o1 o1' /\ distinct_ops o1 ol /\ distinct_ops o1' ol /\
                     ~ (get_key o1 = get_key o1' /\ get_key o1 = get_key ol /\
@@ -714,11 +891,13 @@ let ind_left_1op (l a b:concrete_st) (o1 o1' ol:op_t)
                     eq (merge (do l ol) (do a o1) (do b ol)) (do (merge (do l ol) a (do b ol)) o1))
           (ensures eq (merge (do l ol) (do (do a o1') o1) (do b ol)) (do (merge (do l ol) (do a o1') (do b ol)) o1)) = 
   let k = get_key ol in
-  let ka = Alpha_t k in let kb = Beta_t k in
+  let ka = Alpha_t k in let kb = Beta_t k in let kc = Gamma_t k in
   if get_key o1 = k && get_key o1' = k && is_alpha_op o1 && is_alpha_op o1' && is_alpha_op ol then
       ind_left_1op_a (sel l ka) (sel a ka) (sel b ka) (get_op_a o1) (get_op_a o1') (get_op_a ol)
   else if get_key o1 = k && get_key o1' = k && is_beta_op o1 && is_beta_op o1' && is_beta_op ol then
       ind_left_1op_b (sel l kb) (sel a kb) (sel b kb) (get_op_b o1) (get_op_b o1') (get_op_b ol)
+  else if get_key o1 = k && get_key o1' = k && is_gamma_op o1 && is_gamma_op o1' && is_gamma_op ol then
+      ind_left_1op_c (sel l kc) (sel a kc) (sel b kc) (get_op_c o1) (get_op_c o1') (get_op_c ol)
   else ind_left_1op' l a b o1 o1' ol
 
 (*Zero OP*)
@@ -729,10 +908,14 @@ val lem_0op_a (l a b:concrete_st_a) (ol:op_a)
 val lem_0op_b (l a b:concrete_st_b) (ol:op_b)
   : Lemma (ensures eq_b (merge_b (do_b l ol) (do_b a ol) (do_b b ol)) (do_b (merge_b l a b) ol))
 
+val lem_0op_c (l a b:concrete_st_c) (ol:op_c)
+  : Lemma (ensures eq_c (merge_c (do_c l ol) (do_c a ol) (do_c b ol)) (do_c (merge_c l a b) ol))
+  
 let lem_0op (l a b:concrete_st) (ol:op_t)
   : Lemma (ensures eq (merge (do l ol) (do a ol) (do b ol)) (do (merge l a b) ol)) =
   let k = get_key ol in
-  let ka = Alpha_t k in let kb = Beta_t k in
+  let ka = Alpha_t k in let kb = Beta_t k in let kc = Gamma_t k in
   if is_alpha_op ol then lem_0op_a (sel l ka) (sel a ka) (sel b ka) (get_op_a ol)
   else if is_beta_op ol then lem_0op_b (sel l kb) (sel a kb) (sel b kb) (get_op_b ol)
+  else if is_gamma_op ol then lem_0op_c (sel l kc) (sel a kc) (sel b kc) (get_op_c ol)
   else ()
