typeclass/Json.fst
@@ -1,8 +1,16 @@
-module Library
+module Json
 
 open FStar.Seq
+module M = Dependent_map
+module S = Set_extended
 
+type kt : eqtype =
+  |Alpha_t : string -> kt
+  |Beta_t : string -> kt
+  
 let get_rid (_,(rid,_)) = rid
+
+type log = seq (pos & (nat & eqtype))
 
 //conflict resolution type
 type rc_res =
@@ -27,10 +35,10 @@ type op (#o:eqtype) = pos (*timestamp*) & (nat (*replica ID*) & o)
 let distinct_ops (op1 op2:op) = fst op1 =!= fst op2
 
 val apply_log : #st:Type0 -> #o:eqtype -> {|mrdt st o|} -> s:st -> l:seq (pos & (nat & o)) -> Tot st
-let rec apply_log #st #o #m (s:st) (l:seq (pos & (nat & o))) : Tot st (decreases length l) =
+let rec apply_log #st #o #m s l : Tot st (decreases length l) =
   match length l with
   |0 -> s
-  |_ -> apply_log #st #o #m (m.do s (head l)) (tail l) 
+  |_ -> apply_log (do #st #o s (head l)) (tail l) 
 
 class cond (st:Type0) (app_op:eqtype) (m:mrdt st app_op) = {
   rc_non_comm : o1:op -> o2:op ->
@@ -53,7 +61,6 @@ class cond (st:Type0) (app_op:eqtype) (m:mrdt st app_op) = {
           (ensures m.eq (m.do (m.do (apply_log (m.do (m.do s o1) o2) l) o) o3) (m.do (m.do (apply_log (m.do (m.do s o2) o1) l) o) o3))         
 }
 
-
 class vc (st:Type0) (app_op:eqtype) (m:mrdt st app_op) = {
   merge_comm : l:st -> a:st -> b:st ->
     Lemma (ensures (m.eq (m.merge l a b) (m.merge l b a)));
@@ -63,15 +70,16 @@ class vc (st:Type0) (app_op:eqtype) (m:mrdt st app_op) = {
 
   base_2op : o1:op -> o2:op ->
     Lemma (requires (Fst_then_snd? (m.rc o2 o1) \/ Either? (m.rc o2 o1)) /\ get_rid o1 <> get_rid o2 /\ distinct_ops o1 o2)
-          (ensures m.eq (m.merge m.init_st (m.do m.init_st o1) (m.do m.init_st o2)) 
-                        (m.do (m.merge m.init_st m.init_st (m.do m.init_st o2)) o1));
+          (ensures m.eq (m.merge m.init_st (m.do m.init_st o1) (m.do m.init_st o2)) (m.do (m.merge m.init_st m.init_st (m.do m.init_st o2)) o1));
 
   ind_lca_2op : l:st -> o1:op -> o2:op -> ol:op ->
   Lemma (requires (Fst_then_snd? (m.rc o2 o1) \/ Either? (m.rc o2 o1)) /\
-                  get_rid o1 <> get_rid o2 /\ distinct_ops o1 o2 /\ distinct_ops o1 ol /\ distinct_ops o2 ol /\
+                  get_rid o1 <> get_rid o2 /\
+                  distinct_ops o1 o2 /\
+                  distinct_ops o1 ol /\
+                  distinct_ops o2 ol /\
                   m.eq (m.merge l (m.do l o1) (m.do l o2)) (m.do (m.merge l l (m.do l o2)) o1))
-        (ensures m.eq (m.merge (m.do l ol) (m.do (m.do l ol) o1) (m.do (m.do l ol) o2)) 
-                      (m.do (m.merge (m.do l ol) (m.do l ol) (m.do (m.do l ol) o2)) o1));
+        (ensures m.eq (m.merge (m.do l ol) (m.do (m.do l ol) o1) (m.do (m.do l ol) o2)) (m.do (m.merge (m.do l ol) (m.do l ol) (m.do (m.do l ol) o2)) o1));
 
   inter_right_base_2op : l:st -> a:st -> b:st -> o1:op -> o2:op -> ob:op -> ol:op ->
   Lemma (requires (Fst_then_snd? (m.rc o2 o1) \/ Either? (m.rc o2 o1)) /\ Fst_then_snd? (m.rc ob ol) /\
@@ -121,13 +129,19 @@ inter_left_2op : l:st -> a:st -> b:st -> o1:op -> o2:op -> ob:op -> ol:op -> o:o
 
 ind_right_2op : l:st -> a:st -> b:st -> o1:op -> o2:op -> o2':op ->
   Lemma (requires Fst_then_snd? (m.rc o2 o1) /\
-                  get_rid o1 <> get_rid o2 /\ distinct_ops o1 o2 /\ distinct_ops o1 o2' /\ distinct_ops o2 o2' /\
+                  get_rid o1 <> get_rid o2 /\
+                  distinct_ops o1 o2 /\
+                  distinct_ops o1 o2' /\
+                  distinct_ops o2 o2' /\
                   m.eq (m.merge l (m.do a o1) (m.do b o2)) (m.do (m.merge l a (m.do b o2)) o1))
         (ensures m.eq (m.merge l (m.do a o1) (m.do (m.do b o2') o2)) (m.do (m.merge l a (m.do (m.do b o2') o2)) o1));
 
 ind_left_2op : l:st -> a:st -> b:st -> o1:op -> o2:op -> o1':op ->
   Lemma (requires (Fst_then_snd? (m.rc o2 o1) \/ Either? (m.rc o2 o1)) /\
-                  get_rid o1 <> get_rid o2 /\ distinct_ops o1 o2 /\ distinct_ops o1 o1' /\ distinct_ops o2 o1' /\
+                  get_rid o1 <> get_rid o2 /\
+                  distinct_ops o1 o2 /\
+                  distinct_ops o1 o1' /\
+                  distinct_ops o2 o1' /\
                   m.eq (m.merge l (m.do a o1) (m.do b o2)) (m.do (m.merge l a (m.do b o2)) o1))
         (ensures m.eq (m.merge l (m.do (m.do a o1') o1) (m.do b o2)) (m.do (m.merge l (m.do a o1') (m.do b o2)) o1));
 
@@ -141,48 +155,42 @@ ind_lca_1op : l:st -> o1:op -> ol:op ->
 
 inter_right_base_1op : l:st -> a:st -> b:st -> o1:op -> ob:op -> ol:op ->
   Lemma (requires Fst_then_snd? (m.rc ob ol) /\ get_rid ob <> get_rid ol /\
-                  distinct_ops o1 ob /\ distinct_ops o1 ol /\ distinct_ops ob ol /\
-                  (Fst_then_snd? (m.rc ob o1) ==> m.eq (m.merge l (m.do a o1) (m.do b ob)) (m.do (m.merge l a (m.do b ob)) o1)) /\
-                  m.eq (m.merge (m.do l ol) (m.do (m.do a ol) o1) (m.do b ol)) (m.do (m.merge (m.do l ol) (m.do a ol) (m.do b ol)) o1))
-        (ensures m.eq (m.merge (m.do l ol) (m.do (m.do a ol) o1) (m.do (m.do b ob) ol)) 
-                      (m.do (m.merge (m.do l ol) (m.do a ol) (m.do (m.do b ob) ol)) o1));
+                    distinct_ops o1 ob /\ distinct_ops o1 ol /\ distinct_ops ob ol /\
+                    (Fst_then_snd? (m.rc ob o1) ==> m.eq (m.merge l (m.do a o1) (m.do b ob)) (m.do (m.merge l a (m.do b ob)) o1)) /\
+                    m.eq (m.merge (m.do l ol) (m.do (m.do a ol) o1) (m.do b ol)) (m.do (m.merge (m.do l ol) (m.do a ol) (m.do b ol)) o1))
+          (ensures m.eq (m.merge (m.do l ol) (m.do (m.do a ol) o1) (m.do (m.do b ob) ol)) (m.do (m.merge (m.do l ol) (m.do a ol) (m.do (m.do b ob) ol)) o1));
 
 inter_left_base_1op : l:st -> a:st -> b:st -> o1:op -> ob:op -> ol:op ->
   Lemma (requires Fst_then_snd? (m.rc ob ol) /\ get_rid ob <> get_rid ol /\
-                  distinct_ops o1 ob /\ distinct_ops o1 ol /\ distinct_ops ob ol /\
-                  m.eq (m.merge (m.do l ol) (m.do (m.do a ol) o1) (m.do b ol)) (m.do (m.merge (m.do l ol) (m.do a ol) (m.do b ol)) o1))
-        (ensures m.eq (m.merge (m.do l ol) (m.do (m.do (m.do a ob) ol) o1) (m.do b ol)) 
-                      (m.do (m.merge (m.do l ol) (m.do (m.do a ob) ol) (m.do b ol)) o1));
+                    distinct_ops o1 ob /\ distinct_ops o1 ol /\ distinct_ops ob ol /\
+                    m.eq (m.merge (m.do l ol) (m.do (m.do a ol) o1) (m.do b ol)) (m.do (m.merge (m.do l ol) (m.do a ol) (m.do b ol)) o1))
+          (ensures m.eq (m.merge (m.do l ol) (m.do (m.do (m.do a ob) ol) o1) (m.do b ol)) (m.do (m.merge (m.do l ol) (m.do (m.do a ob) ol) (m.do b ol)) o1));
           
 inter_right_1op : l:st -> a:st -> b:st -> o1:op -> ob:op -> ol:op -> o:op ->
   Lemma (requires Fst_then_snd? (m.rc ob ol) /\ get_rid ob <> get_rid ol /\
-                  (~ (Either? (m.rc o ob)) \/ Fst_then_snd? (m.rc o ol)) /\
-                  distinct_ops o1 ob /\ distinct_ops o1 ol /\ distinct_ops o1 o /\ distinct_ops ob ol /\ distinct_ops ob o /\ distinct_ops ol o /\
-                  get_rid o <> get_rid ol /\
-                  m.eq (m.merge (m.do l ol) (m.do (m.do a ol) o1) (m.do (m.do b ob) ol)) 
-                       (m.do (m.merge (m.do l ol) (m.do a ol) (m.do (m.do b ob) ol)) o1))
-        (ensures m.eq (m.merge (m.do l ol) (m.do (m.do a ol) o1) (m.do (m.do (m.do b o) ob) ol)) 
-                      (m.do (m.merge (m.do l ol) (m.do a ol) (m.do (m.do (m.do b o) ob) ol)) o1));
+                    (~ (Either? (m.rc o ob)) \/ Fst_then_snd? (m.rc o ol)) /\
+                    distinct_ops o1 ob /\ distinct_ops o1 ol /\ distinct_ops o1 o /\ distinct_ops ob ol /\ distinct_ops ob o /\ distinct_ops ol o /\
+                    get_rid o <> get_rid ol /\
+                    m.eq (m.merge (m.do l ol) (m.do (m.do a ol) o1) (m.do (m.do b ob) ol)) (m.do (m.merge (m.do l ol) (m.do a ol) (m.do (m.do b ob) ol)) o1))
+          (ensures m.eq (m.merge (m.do l ol) (m.do (m.do a ol) o1) (m.do (m.do (m.do b o) ob) ol)) (m.do (m.merge (m.do l ol) (m.do a ol) (m.do (m.do (m.do b o) ob) ol)) o1));
 
 inter_left_1op : l:st -> a:st -> b:st -> o1:op -> ob:op -> ol:op -> o:op ->
   Lemma (requires Fst_then_snd? (m.rc ob ol) /\ get_rid ob <> get_rid ol /\
-                  (~ (Either? (m.rc o ob)) \/ Fst_then_snd? (m.rc o ol)) /\
-                  distinct_ops o1 ob /\ distinct_ops o1 ol /\ distinct_ops o1 o /\ distinct_ops ob ol /\ distinct_ops ob o /\ distinct_ops ol o /\
-                  get_rid o <> get_rid ol /\
-                  m.eq (m.merge (m.do l ol) (m.do (m.do (m.do a ob) ol) o1) (m.do b ol)) 
-                       (m.do (m.merge (m.do l ol) (m.do (m.do a ob) ol) (m.do b ol)) o1))
-        (ensures m.eq (m.merge (m.do l ol) (m.do (m.do (m.do (m.do a o) ob) ol) o1) (m.do b ol)) 
-                      (m.do (m.merge (m.do l ol) (m.do (m.do (m.do a o) ob) ol) (m.do b ol)) o1));
+                    (~ (Either? (m.rc o ob)) \/ Fst_then_snd? (m.rc o ol)) /\
+                    distinct_ops o1 ob /\ distinct_ops o1 ol /\ distinct_ops o1 o /\ distinct_ops ob ol /\ distinct_ops ob o /\ distinct_ops ol o /\
+                    get_rid o <> get_rid ol /\
+                    m.eq (m.merge (m.do l ol) (m.do (m.do (m.do a ob) ol) o1) (m.do b ol)) (m.do (m.merge (m.do l ol) (m.do (m.do a ob) ol) (m.do b ol)) o1))
+          (ensures m.eq (m.merge (m.do l ol) (m.do (m.do (m.do (m.do a o) ob) ol) o1) (m.do b ol)) (m.do (m.merge (m.do l ol) (m.do (m.do (m.do a o) ob) ol) (m.do b ol)) o1));
 
 ind_left_1op : l:st -> a:st -> b:st -> o1:op -> o1':op -> ol:op ->
   Lemma (requires distinct_ops o1 o1' /\ distinct_ops o1 ol /\ distinct_ops o1' ol /\
-                  m.eq (m.merge (m.do l ol) (m.do a o1) (m.do b ol)) (m.do (m.merge (m.do l ol) a (m.do b ol)) o1))
-        (ensures m.eq (m.merge (m.do l ol) (m.do (m.do a o1') o1) (m.do b ol)) (m.do (m.merge (m.do l ol) (m.do a o1') (m.do b ol)) o1));
+                    m.eq (m.merge (m.do l ol) (m.do a o1) (m.do b ol)) (m.do (m.merge (m.do l ol) a (m.do b ol)) o1))
+          (ensures m.eq (m.merge (m.do l ol) (m.do (m.do a o1') o1) (m.do b ol)) (m.do (m.merge (m.do l ol) (m.do a o1') (m.do b ol)) o1));
 
 ind_right_1op : l:st -> a:st -> b:st -> o2:op -> o2':op -> ol:op ->
   Lemma (requires distinct_ops o2 o2' /\ distinct_ops o2 ol /\ distinct_ops o2' ol /\
-                  m.eq (m.merge (m.do l ol) (m.do a ol) (m.do b o2)) (m.do (m.merge (m.do l ol) (m.do a ol) b) o2))
-        (ensures m.eq (m.merge (m.do l ol) (m.do a ol) (m.do (m.do b o2') o2)) (m.do (m.merge (m.do l ol) (m.do a ol) (m.do b o2')) o2));
+                    m.eq (m.merge (m.do l ol) (m.do a ol) (m.do b o2)) (m.do (m.merge (m.do l ol) (m.do a ol) b) o2))
+          (ensures m.eq (m.merge (m.do l ol) (m.do a ol) (m.do (m.do b o2') o2)) (m.do (m.merge (m.do l ol) (m.do a ol) (m.do b o2')) o2));
 
 lem_0op : l:st -> a:st -> b:st -> ol:op ->
   Lemma (ensures m.eq (m.merge (m.do l ol) (m.do a ol) (m.do b ol)) (m.do (m.merge l a b) ol))
